efsm-ltl/EFSM_LTL.thy
@@ -1,0 +1,276 @@
+theory EFSM_LTL                                                     
+imports "../EFSM" "HOL-Library.Linear_Temporal_Logic_on_Streams"
+begin
+
+record state =
+  statename :: "nat option"
+  datastate :: registers
+  event :: event
+  "output" :: outputs
+
+type_synonym property = "state stream \<Rightarrow> bool"
+
+abbreviation label :: "state \<Rightarrow> String.literal" where
+  "label s \<equiv> fst (event s)"
+
+abbreviation inputs :: "state \<Rightarrow> value list" where
+  "inputs s \<equiv> snd (event s)"
+
+fun ltl_step :: "transition_matrix \<Rightarrow> nat option \<Rightarrow> registers \<Rightarrow> event \<Rightarrow> (nat option \<times> outputs \<times> registers)" where
+  "ltl_step _ None r _ = (None, [], r)" |
+  "ltl_step e (Some s) r (l, i) = (let possibilities = possible_steps e s r l i in
+                   if possibilities = {||} then (None, [], r)
+                   else
+                     let (s', t) = Eps (\<lambda>x. x |\<in>| possibilities) in
+                     (Some s', (apply_outputs (Outputs t) (join_ir i r)), (apply_updates (Updates t) (join_ir i r) r))
+                  )"
+
+lemma ltl_step_alt:  "ltl_step e (Some s) r t = (let possibilities = possible_steps e s r (fst t) (snd t) in
+                   if possibilities = {||} then (None, [], r)
+                   else
+                     let (s', t') = Eps (\<lambda>x. x |\<in>| possibilities) in
+                     (Some s', (apply_outputs (Outputs t') (join_ir (snd t) r)), (apply_updates (Updates t') (join_ir (snd t) r) r))
+                  )"
+  apply (case_tac t)
+  by (simp add: Let_def)
+
+lemma ltl_step_none: "possible_steps e s r (fst ie) (snd ie) = {||} \<Longrightarrow> ltl_step e (Some s) r ie = (None, [], r)"
+  by (simp add: ltl_step_alt)
+
+primcorec make_full_observation :: "transition_matrix \<Rightarrow> nat option \<Rightarrow> registers \<Rightarrow> outputs \<Rightarrow> event stream \<Rightarrow> state stream" where
+  "make_full_observation e s d p i = (
+    let (s', o', d') = ltl_step e s d (shd i) in
+    \<lparr>statename = s, datastate = d, event=(shd i), output = p\<rparr>##(make_full_observation e s' d' o' (stl i))
+  )"
+
+definition watch :: "transition_matrix \<Rightarrow> event stream \<Rightarrow> state stream" where
+  "watch e i \<equiv> (make_full_observation e (Some 0) <> [] i)"
+
+definition state_eq :: "nat option \<Rightarrow> state stream \<Rightarrow> bool" where
+  "state_eq v s \<equiv> statename (shd s) = v"
+
+lemma state_eq_holds: "state_eq s = holds (\<lambda>x. statename x = s)"
+  apply (rule ext)
+  by (simp add: state_eq_def holds_def)
+
+lemma state_eq_None_not_Some: "state_eq None s \<Longrightarrow> \<not> state_eq (Some n) s"
+  by (simp add: state_eq_def)
+
+definition label_eq :: "string \<Rightarrow> state stream \<Rightarrow> bool" where
+  "label_eq v s \<equiv> fst (event (shd s)) = (String.implode v)"
+
+lemma watch_label: "label_eq l (watch e t) = (fst (shd t) = String.implode l)"
+  by (simp add: label_eq_def watch_def)
+
+definition input_eq :: "value list \<Rightarrow> state stream \<Rightarrow> bool" where
+  "input_eq v s \<equiv> inputs (shd s) = v"
+
+definition event_eq :: "(string \<times> inputs) \<Rightarrow> state stream \<Rightarrow> bool" where
+  "event_eq e = label_eq (fst e) aand input_eq (snd e)"
+
+lemmas event_eq = event_eq_def label_eq_def input_eq_def
+
+definition output_eq :: "value option list \<Rightarrow> state stream \<Rightarrow> bool" where
+  "output_eq v s \<equiv> output (shd s) = v"
+
+lemma shd_state_is_none: "(state_eq None) (make_full_observation e None r p t)"
+  by (simp add: state_eq_def)
+
+lemma unfold_observe_none: "make_full_observation e None d p t = (\<lparr>statename = None, datastate = d, event=(shd t), output = p\<rparr>##(make_full_observation e None d [] (stl t)))"
+  by (simp add: stream.expand)
+
+lemma once_none_always_none: "alw (state_eq None) (make_full_observation e None r p t)"
+proof -
+  obtain ssa :: "((String.literal \<times> value list) stream \<Rightarrow> state stream) \<Rightarrow> (String.literal \<times> value list) stream" where
+      "\<forall>f p s. f (stl (ssa f)) \<noteq> stl (f (ssa f)) \<or> alw p (f s) = alw (\<lambda>s. p (f s)) s"
+    by (metis (no_types) alw_inv)
+  then have "alw (state_eq None) (make_full_observation e None r [] (stl t))"
+    by (metis (no_types) all_imp_alw shd_state_is_none stream.sel(2) unfold_observe_none)
+  then show ?thesis
+    by (metis (no_types) alw.simps shd_state_is_none stream.sel(2) unfold_observe_none)
+qed
+
+lemma once_none_nxt_always_none: "alw (nxt (state_eq None)) (make_full_observation e None r p t)"
+proof(coinduction)
+  case alw
+  then show ?case
+    apply simp
+    by (metis alw_iff_sdrop nxt.simps once_none_always_none sdrop_simps(2) shd_state_is_none)
+qed
+
+lemma no_output_none: "nxt (alw (output_eq [])) (make_full_observation e None r p t)"
+proof -
+  obtain ss :: "((String.literal \<times> value list) stream \<Rightarrow> state stream) \<Rightarrow> (String.literal \<times> value list) stream" where
+    "\<forall>f p s. f (stl (ss f)) \<noteq> stl (f (ss f)) \<or> alw p (f s) = alw (\<lambda>s. p (f s)) s"
+    by (metis (no_types) alw_inv)
+  then show ?thesis
+    by (simp add: output_eq_def all_imp_alw)
+qed
+
+lemma no_output_none_nxt: "alw (nxt (output_eq [])) (make_full_observation e None r p t)"
+  by (metis alw_inv alw_mono no_output_none nxt.simps)
+
+lemma no_updates_none: "alw (\<lambda>x. datastate (shd x) = r) (make_full_observation e None r p t)"
+proof -
+  have "alw (\<lambda>x. datastate (shd x) = r) (make_full_observation e None r [] (stl t))"
+    proof -
+      obtain ss :: "((String.literal \<times> value list) stream \<Rightarrow> state stream) \<Rightarrow> (String.literal \<times> value list) stream" where
+        "\<forall>f p s. f (stl (ss f)) \<noteq> stl (f (ss f)) \<or> alw p (f s) = alw (\<lambda>s. p (f s)) s"
+        by (metis (no_types) alw_inv)
+      then show ?thesis
+        by (simp add: output_eq_def all_imp_alw)
+    qed
+    then show ?thesis
+    proof(coinduction)
+      case alw
+      then show ?case
+        by simp
+    qed
+qed
+
+lemma event_components: "(label_eq l aand input_eq i) s = (event (shd s) = (String.implode l, i))"
+  apply (simp add: label_eq_def input_eq_def)
+  by (metis fst_conv prod.collapse snd_conv)
+
+lemma alw_not_some: "alw (\<lambda>xs. statename (shd xs) \<noteq> Some s) (make_full_observation e None r p t)"
+  by (metis (mono_tags, lifting) alw_mono once_none_always_none option.distinct(1) state_eq_def)
+
+lemma state_none: "((state_eq None) impl nxt (state_eq None)) (make_full_observation e s r p t)"
+  by (simp add: state_eq_def)
+
+lemma state_none_2: "(state_eq None) (make_full_observation e s r p t) \<Longrightarrow> (state_eq None) (make_full_observation e s r p (stl t))"
+  by (simp add: state_eq_def)
+
+lemma decompose_pair: "e \<noteq> (l, i) = (\<not> (fst e =l \<and> snd e = i))"
+  by (metis fst_conv prod.collapse sndI)
+
+datatype ltl_vname = Ip nat | Op nat | Rg nat
+
+type_synonym ltl_gexp = "ltl_vname gexp"
+
+definition join_iro :: "value list \<Rightarrow> registers \<Rightarrow> outputs \<Rightarrow> ltl_vname datastate" where
+  "join_iro i r p = (\<lambda>x. case x of
+    Rg n \<Rightarrow> r $ n |
+    Ip n \<Rightarrow> Some (i ! n) |
+    Op n \<Rightarrow> p ! n
+  )"
+
+lemma join_iro_R [simp]: "join_iro i r p (Rg n) = r $ n"
+  by (simp add: join_iro_def)
+
+definition check_exp :: "ltl_gexp \<Rightarrow> state stream \<Rightarrow> bool" where
+  "check_exp g s = (gval g (join_iro (snd (event (shd s))) (datastate (shd s)) (output (shd s))) = trilean.true)"
+
+lemma alw_ev: "alw f = not (ev (\<lambda>s. \<not>f s))"
+  by simp
+
+lemma stream_eq_scons: "shd x = h \<Longrightarrow> stl x = t \<Longrightarrow> x = h##t"
+  by auto
+
+lemma alw_state_eq_smap: "alw (state_eq s) ss = alw (\<lambda>ss. shd ss = s) (smap statename ss)"
+  apply standard
+   apply (simp add: alw_iff_sdrop state_eq_def)
+  by (simp add: alw_mono alw_smap state_eq_def)
+
+lemma alw_holds: "alw (holds P) (h##t) = (P h \<and> alw (holds P) t)"
+  apply standard
+   apply auto[1]
+  by (metis alw.simps holds_Stream stream.sel(2))
+
+lemma alw_holds2: "alw (holds P) ss = (P (shd ss) \<and> alw (holds P) (stl ss))"
+  by (meson alw.simps holds.elims(2) holds.elims(3))
+
+lemma snth_sconst: "(\<forall>i. s !! i = h) = (s = sconst h)"
+  by (metis funpow_code_def id_funpow sdrop_simps(1) sdrop_siterate siterate.simps(1) smap_alt smap_sconst snth.simps(1) stream.map_id)
+
+lemma alw_sconst: "(alw (\<lambda>xs. shd xs = h) t) = (t = sconst h)"
+  by (simp add: snth_sconst[symmetric] alw_iff_sdrop)
+
+lemma smap_statename_None: "smap statename (make_full_observation e None r p i) = sconst None"
+  by (meson EFSM_LTL.alw_sconst alw_state_eq_smap once_none_always_none)
+
+(* Out of interest, Nitpick finds a spurious counterexample to this *)
+lemma sdrop_if_suntil: "(p suntil q) \<omega> \<Longrightarrow> \<exists>j. q (sdrop j \<omega>) \<and> (\<forall>k < j. p (sdrop k \<omega>))"
+proof(induction rule: suntil.induct)
+  case (base \<omega>)
+then show ?case
+  by force
+next
+  case (step \<omega>)
+  then show ?case
+    apply clarify
+    apply (rule_tac x="j+1" in exI)
+    apply simp
+    using ev_at_imp_snth less_Suc_eq_0_disj by auto
+qed
+
+lemma suntil_implies_until: "(\<phi> suntil \<psi>) \<omega> \<Longrightarrow> (\<phi> until \<psi>) \<omega>"
+  by (simp add: UNTIL.base UNTIL.step suntil_induct_strong)
+
+lemma alw_implies_until: "alw \<phi> \<omega> \<Longrightarrow> (\<phi> until \<psi>) \<omega>"
+  by (metis until_false until_mono)
+
+lemma until_ev_suntil: "ev \<psi> \<omega> \<Longrightarrow> (\<phi> until \<psi>) \<omega> \<Longrightarrow> (\<phi> suntil \<psi>) \<omega>"
+proof(induction rule: ev.induct)
+  case (base xs)
+  then show ?case
+    by (simp add: suntil.base)
+next
+  case (step xs)
+  then show ?case
+    by (metis UNTIL.cases suntil.base suntil.step)
+qed
+
+lemma suntil_as_until: "(\<phi> suntil \<psi>) \<omega> = ((\<phi> until \<psi>) \<omega> \<and> ev \<psi> \<omega>)"
+  using ev_suntil suntil_implies_until until_ev_suntil by blast
+
+lemma not_relesased_yet: "(\<phi> until \<psi>) \<omega> \<Longrightarrow> \<not> \<psi> \<omega> \<Longrightarrow> \<phi> \<omega>"
+  using UNTIL.cases by auto
+
+lemma until_must_release: "ev (not \<phi>) \<omega> \<Longrightarrow> (\<phi> until \<psi>) \<omega> \<Longrightarrow> ev \<psi> \<omega>"
+proof(induction rule: ev.induct)
+  case (base xs)
+  then show ?case
+    using not_relesased_yet by blast
+next
+  case (step xs)
+  then show ?case
+    using UNTIL.cases by blast
+qed
+
+lemma until_as_suntil: "(\<phi> until \<psi>) \<omega> = ((\<phi> suntil \<psi>) or (alw \<phi>)) \<omega>"
+  using alw_implies_until not_alw_iff suntil_implies_until until_ev_suntil until_must_release by blast
+
+lemma not_suntil: "(\<not> (p suntil q) \<omega>) = (\<not> (p until q) \<omega> \<or> alw (not q) \<omega>)"
+  by (simp add: suntil_as_until alw_iff_sdrop ev_iff_sdrop)
+
+lemma "(p until q) \<omega> = (q \<omega> \<or> (p \<omega> \<and> (p until q) (stl \<omega>)))"
+  using UNTIL.simps by auto
+
+lemma stl_as_sdrop: "stl s = sdrop 1 s"
+  by simp
+
+lemma less_suc: "(\<forall>k<Suc j. p (sdrop k \<omega>)) = ((\<forall>k< j. p (sdrop k \<omega>)) \<and> p (sdrop j \<omega>))"
+  using less_Suc_eq by auto
+
+lemma sdrop_until: "q (sdrop j \<omega>) \<Longrightarrow> \<forall>k<j. p (sdrop k \<omega>) \<Longrightarrow> (p until q) \<omega>"
+proof(induct j arbitrary: \<omega>)
+  case 0
+  then show ?case
+    by (simp add: UNTIL.base)
+next
+  case (Suc j)
+  then show ?case
+    by (metis Suc_mono UNTIL.simps sdrop.simps(1) sdrop.simps(2) zero_less_Suc)
+qed
+
+lemma sdrop_suntil: "q (sdrop j \<omega>) \<Longrightarrow> (\<forall>k < j. p (sdrop k \<omega>)) \<Longrightarrow> (p suntil q) \<omega>"
+  apply (simp add: suntil_as_until conj_commute)
+  apply standard
+   apply (simp add: nxt_ev nxt_sdrop)
+  by (simp add: sdrop_until)
+
+lemma sdrop_iff_suntil: "(p suntil q) \<omega> = (\<exists>j. q (sdrop j \<omega>) \<and> (\<forall>k < j. p (sdrop k \<omega>)))"
+  using sdrop_if_suntil sdrop_suntil by blast
+
+end
