efsm-ltl/LTL_Exp.thy
@@ -1,0 +1,21 @@
+theory LTL_Exp
+imports Main "../EFSM" FinFun.FinFun
+begin
+
+no_notation relcomp (infixr "O" 75) and comp (infixl "o" 55)
+
+datatype ltl_vname = Ip nat | Op nat | Rg nat
+
+type_synonym ltl_gexp = "ltl_vname gexp"
+
+definition join_iro :: "value list \<Rightarrow> registers \<Rightarrow> outputs \<Rightarrow> ltl_vname datastate" where
+  "join_iro i r o = (\<lambda>x. case x of
+    Rg n \<Rightarrow> r $ n |
+    Ip n \<Rightarrow> Some (i ! n) |
+    Op n \<Rightarrow> o ! n
+  )"
+
+lemma join_iro_R [simp]: "join_iro i r o (Rg n) = r $ n"
+  by (simp add: join_iro_def)
+
+end
