examples/Drinks_Machine.thy
@@ -12,8 +12,10 @@ states. The fourth element is included here so that the \emph{statename} datatyp
 the next example.
 \<close>
 theory Drinks_Machine
-  imports "../Contexts"
+  imports "../efsm-ltl/EFSM_LTL"
 begin
+
+declare One_nat_def [simp del]
 
 definition select :: "transition" where
 "select \<equiv> \<lparr>
@@ -41,9 +43,6 @@ definition coin :: "transition" where
       \<rparr>"
 text_raw\<open>}%endsnip\<close>
 
-lemma label_coin: "Label coin = STR ''coin''"
-  by (simp add: coin_def)
-
 definition vend :: "transition" where
 "vend \<equiv> \<lparr>
         Label = STR ''vend'',
@@ -52,9 +51,6 @@ definition vend :: "transition" where
         Outputs =  [(V (R 1))],
         Updates = [(1, V (R 1)), (2, V (R 2))]
       \<rparr>"
-
-lemma label_vend: "Label vend = STR ''vend''"
-  by (simp add: vend_def)
 
 definition vend_fail :: "transition" where
 "vend_fail \<equiv> \<lparr>
@@ -65,12 +61,6 @@ definition vend_fail :: "transition" where
         Updates = [(1, V (R 1)), (2, V (R 2))]
       \<rparr>"
 
-lemma label_vend_fail: "Label vend_fail = STR ''vend''"
-  by (simp add: vend_fail_def)
-
-lemma arity_vend_fail: "Arity vend_fail = 0"
-  by (simp add: vend_fail_def)
-
 definition drinks :: "transition_matrix" where
 "drinks \<equiv> {|
           ((0,1), select),    \<comment> \<open> If we want to go from state 1 to state 2 then select will do that \<close>
@@ -79,19 +69,16 @@ definition drinks :: "transition_matrix" where
           ((1,2), vend) \<comment> \<open> If we want to go from state 2 to state 3 then vend will do that \<close>
          |}"
 
+lemmas transitions = select_def coin_def vend_def vend_fail_def
+
 lemma "S drinks = {|0, 1, 2|}"
   apply (simp add: S_def drinks_def)
   by auto
-
-lemmas transitions = select_def coin_def vend_def vend_fail_def
 
 lemma possible_steps_0:  "length i = 1 \<Longrightarrow> possible_steps drinks 0 r (STR ''select'') i = {|(1, select)|}"
   apply (simp add: possible_steps_singleton drinks_def)
   apply safe
   by (simp_all add: transitions apply_guards_def)
-
-lemma arity_vend: "Arity vend = 0"
-  by (simp add: vend_def)
 
 lemma drinks_vend_insufficient: "r $ 2 = Some (Num x1) \<Longrightarrow> x1 < 100 \<Longrightarrow> possible_steps drinks 1 r (STR ''vend'') [] = {|(1, vend_fail)|}"
   apply (simp add: possible_steps_singleton drinks_def)
@@ -99,37 +86,33 @@ lemma drinks_vend_insufficient: "r $ 2 = Some (Num x1) \<Longrightarrow> x1 < 10
   by (simp_all add: transitions apply_guards_def value_gt_def join_ir_def connectives)
 
 lemma drinks_vend_invalid: "\<nexists>n. r $ 2 = Some (Num n) \<Longrightarrow> possible_steps drinks 1 r (STR ''vend'') [] = {||}"
-  apply (simp add: possible_steps_empty drinks_def)
-  apply safe
-  by (simp_all add: transitions apply_guards_def join_ir_def value_gt_def MaybeBoolInt_not_num_1 connectives)
+  apply (simp add: possible_steps_empty drinks_def can_take_transition_def can_take_def transitions)
+  by (simp add: MaybeBoolInt_not_num_1 value_gt_def)
 
 lemma possible_steps_1_coin: "length i = 1 \<Longrightarrow> possible_steps drinks 1 r (STR ''coin'') i = {|(1, coin)|}"
   apply (simp add: possible_steps_singleton drinks_def)
   apply safe
-  by (simp_all add: transitions )
+  by (simp_all add: transitions)
 
 lemma possible_steps_2_vend: "\<exists>n. r $ 2 = Some (Num n) \<and> n \<ge> 100 \<Longrightarrow> possible_steps drinks 1 r (STR ''vend'') [] = {|(2, vend)|}"
   apply (simp add: possible_steps_singleton drinks_def)
   apply safe
   by (simp_all add: transitions apply_guards_def value_gt_def join_ir_def connectives)
 
-lemma accepts_from_2: "accepts drinks 1 (<>(2 := Num 100, 1 := d)) [(STR ''vend'', [])]"
+lemma accepts_from_2: "accepts drinks 1 (<>(1 := d, 2 := Num 100)) [(STR ''vend'', [])]"
   apply (rule accepts.step)
   by (simp add: possible_steps_2_vend coin_def join_ir_def input2state_def value_plus_def accepts.base)
 
-lemma regsimp: "<>(2 := n, 1 := d, 2 := n', 1 := d) = <>(2 := n', 1 := d)"
-  by (metis finfun_update_twice finfun_update_twist)
-
-lemma accepts_from_1a: "accepts drinks 1 (<>(2 := Num 50, 1 := d)) [(STR ''coin'', [Num 50]), (STR ''vend'', [])]"
+lemma accepts_from_1a: "accepts drinks 1 (<>(1 := d, 2 := Num 50)) [(STR ''coin'', [Num 50]), (STR ''vend'', [])]"
   apply (rule accepts.step)
-  apply (simp add: possible_steps_1_coin coin_def join_ir_def input2state_def value_plus_def regsimp)
-  by (simp add: accepts_from_2)
+  apply (simp add: possible_steps_1_coin coin_def join_ir_def input2state_def value_plus_def)
+  by (simp add: finfun_update_twist accepts_from_2)
 
 lemma accepts_from_1: "accepts drinks 1 (<>(2 := Num 0, 1 := d))
      [(STR ''coin'', [Num 50]), (STR ''coin'', [Num 50]), (STR ''vend'', [])]"
   apply (rule accepts.step)
-  apply (simp add: possible_steps_1_coin coin_def join_ir_def input2state_def value_plus_def regsimp)
-  by (simp add: accepts_from_1a)
+  apply (simp add: possible_steps_1_coin coin_def join_ir_def input2state_def value_plus_def)
+  by (simp add: finfun_update_twist accepts_from_1a)
 
 lemma purchase_coke: "observe_trace drinks 0 <> [(STR ''select'', [Str ''coke'']), (STR ''coin'', [Num 50]), (STR ''coin'', [Num 50]), (STR ''vend'', [])] =
                        [[], [Some (Num 50)], [Some (Num 100)], [Some (Str ''coke'')]]"
@@ -139,14 +122,14 @@ lemma purchase_coke: "observe_trace drinks 0 <> [(STR ''select'', [Str ''coke'']
     apply (simp add: select_def)
   apply (rule observe_trace_possible_step)
       apply (simp add: possible_steps_1_coin)
-     apply (simp add: coin_def value_plus_def join_ir_def input2state_def regsimp accepts_from_1a)
-    apply (simp add: coin_def value_plus_def join_ir_def input2state_def regsimp apply_outputs_def)
-   apply (simp add: coin_def value_plus_def join_ir_def input2state_def regsimp)
+     apply (simp add: coin_def value_plus_def join_ir_def input2state_def accepts_from_1a)
+    apply (simp add: coin_def value_plus_def join_ir_def input2state_def apply_outputs_def)
+   apply (simp add: coin_def value_plus_def join_ir_def input2state_def)
   apply (rule observe_trace_possible_step)
       apply (simp add: possible_steps_1_coin)
-     apply (simp add: coin_def value_plus_def join_ir_def input2state_def regsimp accepts_from_2)
-    apply (simp add: coin_def value_plus_def join_ir_def input2state_def regsimp apply_outputs_def)
-   apply (simp add: coin_def value_plus_def join_ir_def input2state_def regsimp)
+     apply (simp add: coin_def value_plus_def join_ir_def input2state_def accepts_from_2)
+    apply (simp add: coin_def value_plus_def join_ir_def input2state_def apply_outputs_def)
+   apply (simp add: coin_def value_plus_def join_ir_def input2state_def)
   apply (rule observe_trace_possible_step)
       apply (simp add: possible_steps_2_vend)
      apply (simp add: accepts.base)
@@ -156,8 +139,7 @@ lemma purchase_coke: "observe_trace drinks 0 <> [(STR ''select'', [Str ''coke'']
 
 lemma rejects_input: "l \<noteq> STR ''coin'' \<Longrightarrow> l \<noteq> STR ''vend'' \<Longrightarrow> \<not> accepts drinks 1 d' [(l, i)]"
   apply (rule trace_reject_no_possible_steps)
-  apply (simp add: possible_steps_empty drinks_def)
-  using label_coin label_vend label_vend_fail by blast
+  by (simp add: possible_steps_empty drinks_def can_take_transition_def can_take_def transitions)
 
 lemma rejects_accepts_prefix:
   "l \<noteq> STR ''coin'' \<Longrightarrow>
@@ -171,8 +153,7 @@ lemma rejects_termination: "observe_trace drinks 0 <> [(STR ''select'', [Str ''c
   apply (rule observe_trace_step)
    apply (simp add: step_def possible_steps_0 select_def)
   apply (rule observe_trace_no_possible_step)
-  apply (simp add: possible_steps_def Abs_ffilter Set.filter_def drinks_def)
-  using arity_vend arity_vend_fail label_coin by auto
+  by (simp add: possible_steps_empty drinks_def can_take_transition_def can_take_def transitions)
 
 (* Part of Example 2 in Foster et. al. *)
 lemma r2_0_vend: "can_take_transition vend i r \<Longrightarrow> \<exists>n. r $ 2 = Some (Num n) \<and> n \<ge> 100" (* You can't take vend immediately after taking select *)
@@ -189,17 +170,13 @@ lemma drinks_end: "possible_steps drinks 2 r a b = {||}"
   by force
 
 lemma drinks_vend_r2_String: "r $ 2 = Some (value.Str x2) \<Longrightarrow> possible_steps drinks 1 r (STR ''vend'') [] = {||}"
-  apply (simp add: possible_steps_empty drinks_def)
-  apply safe
-  by (simp_all add: transitions apply_guards_def value_gt_def join_ir_def connectives)
+  apply (simp add: possible_steps_empty drinks_def can_take_transition_def can_take_def transitions)
+  by (simp add: value_gt_def)
 
 lemma drinks_vend_r2_rejects: "\<nexists>n. r $ 2 = Some (Num n) \<Longrightarrow> step drinks 1 r (STR ''vend'') [] = None"
   apply (rule no_possible_steps_1)
-  apply (simp add: possible_steps_empty drinks_def)
-  apply safe
-    apply (simp add: coin_def)
-   apply (simp add: vend_fail_def apply_guards_def join_ir_def value_gt_def MaybeBoolInt_not_num_1 connectives)
-  by (simp add: vend_def apply_guards_def maybe_negate_true maybe_or_false value_gt_def join_ir_def MaybeBoolInt_not_num_1 connectives)
+  apply (simp add: possible_steps_empty drinks_def can_take_transition_def can_take_def transitions)
+  by (simp add: MaybeBoolInt_not_num_1 value_gt_def)
 
 lemma drinks_0_rejects: "\<not> (fst a = STR ''select'' \<and> length (snd a) = 1) \<Longrightarrow>
     (possible_steps drinks 0 r (fst a) (snd a)) = {||}"
@@ -213,27 +190,12 @@ lemma drinks_vend_empty: "(possible_steps drinks 0 <> (STR ''vend'') []) = {||}"
 lemma drinks_1_rejects: "fst a = STR ''coin'' \<longrightarrow> length (snd a) \<noteq> 1 \<Longrightarrow>
           a \<noteq> (STR ''vend'', []) \<Longrightarrow>
           possible_steps drinks 1 r (fst a) (snd a) = {||}"
-proof
-  assume not_coin: "fst a = STR ''coin'' \<longrightarrow> length (snd a) \<noteq> 1"
-  assume not_vend: "a \<noteq> (STR ''vend'', [])"
-  show "possible_steps drinks 1 r (fst a) (snd a) |\<subseteq>| {||}"
-    using not_coin not_vend
-    apply (simp add: drinks_def possible_steps_def)
-    apply safe
-     apply (simp add: One_nat_def)
-    apply (metis arity_vend arity_vend_fail label_coin label_vend label_vend_fail length_0_conv numeral_1_eq_Suc_0 prod.collapse zero_neq_numeral)
-    apply simp
-    by (metis One_nat_def arity_vend arity_vend_fail label_vend label_vend_fail length_0_conv numeral_1_eq_Suc_0 prod.collapse simps(2) transitions(2) zero_neq_numeral)
-  show "{||} |\<subseteq>| possible_steps drinks 1 r (fst a) (snd a)"
-    by simp
-qed
+  apply (simp add: possible_steps_empty drinks_def can_take_transition_def can_take_def transitions)
+  by (metis decompose_pair)
 
-lemma drinks_rejects_future: "t \<noteq> [] \<Longrightarrow> \<not>accepts drinks 2 d t"
-  apply safe
-  apply (rule accepts.cases)
-    apply simp
-   apply simp
-  by (simp add: drinks_end)
+lemma drinks_rejects_future: "rejects drinks 2 d ((l, i)#t)"
+  apply (rule trace_reject_no_possible_steps)
+  by (simp add: possible_steps_empty drinks_def)
 
 lemma drinks_1_rejects_trace: "\<not> (aa = STR ''vend'' \<and> b = []) \<Longrightarrow> \<not> (aa = STR ''coin'' \<and> length b = 1) \<Longrightarrow> \<not>accepts drinks 1 r ((aa, b) # t)"
   apply clarify
@@ -248,11 +210,8 @@ lemma rejects_state_step: "s > 1 \<Longrightarrow> step drinks s r l i = None"
   apply (rule no_possible_steps_1)
   by (simp add: possible_steps_empty drinks_def)
 
-lemma invalid_other_states: "s > 1 \<Longrightarrow> \<not> accepts drinks s r ((aa, b) # t)"
-  apply clarify
-  apply (rule accepts.cases)
-    apply simp
-   apply simp
-  apply clarify
-  using rejects_state_step accepts_cons_step by blast
+lemma invalid_other_states: "s > 1 \<Longrightarrow> rejects drinks s r ((aa, b) # t)"
+  apply (rule trace_reject_no_possible_steps)
+  by (simp add: possible_steps_empty drinks_def)
+
 end
